fast product using the state monad transf. applied to the exception monad
- correctness proof reduced to elementary laws about state and exception monads
- using the primitive mapStateT2 for the state monad transformer
- prove the monad laws for the (non-backtrackable) failstate monad
- add an example that does not backtrack

impredicative_set/iexample_monad_transformer.v
@@ -1,5 +1,6 @@
 From mathcomp Require Import all_ssreflect.
-Require Import imonae_lib ihierarchy imonad_lib ifail_lib istate_lib imonad_transformer imonad_model.
+Require Import imonae_lib ihierarchy imonad_lib ifail_lib istate_lib
+ imonad_transformer imonad_model.
 
 Set Implicit Arguments.
 Unset Strict Implicit.
@@ -106,3 +107,207 @@ End test3.
 End stateTfailMonad.
 
 End example_stateT.
+
+(* The [runStateT] primitive and its laws.
+   To be moved with the definition of the state monad transformer. *)
+Definition runStateT {S A : UU0} {M : monad} (m : stateT S M A) (s : S) :
+M (A*S)%type :=
+m s.
+
+Lemma runStateTFun {S A : UU0} {M : monad} (m : stateT S M A) (s : S) :
+@runStateT _ _ M (fun s => m s) s = m s.
+Proof.
+reflexivity.
+Qed.
+
+Lemma runStateTRet (S A : UU0) (M : monad) (a : A) (s : S) :
+@runStateT _ _ M (Ret a) s = Ret (a, s).
+Proof.
+reflexivity.
+Qed.
+
+Lemma runStateTBind
+  (S A B : UU0) (M : monad) (m : stateT S M A) (f : A -> stateT S M B) (s : S) :
+runStateT (m >>= f) s =
+runStateT m s >>= fun a_s' => runStateT (f (fst a_s')) (snd a_s').
+Proof.
+Admitted.
+
+Lemma runStateTGet (S : UU0) (M : monad) (s : S) :
+@runStateT _ _ M Get s = Ret (s, s).
+Proof.
+Admitted.
+
+Lemma runStateTPut (S : UU0) (M : monad) (s' s : S) :
+@runStateT _ _ M (Put s') s = Ret (tt, s').
+Proof.
+Admitted.
+
+Lemma runStateTLfail (S A : UU0) (M : failMonad) (s : S) :
+runStateT (Lift (stateT S) M A Fail) s = Fail.
+Proof.
+Admitted.
+
+(* No need to unfold [runStateT] later because its laws are sufficient to
+   conclude proofs. *)
+Opaque runStateT.
+
+(* [evalStateT] and [mapStateT2] are not primitives but are defined
+   with [runStateT]. They will be unfolded in proof scripts below in
+   order to apply the laws of [runStateT]. *)
+Definition evalStateT {S A : UU0} {M : monad} (m : stateT S M A) (s : S) :
+M A :=
+runStateT m s >>= fun a_s' => Ret (a_s'.1).
+
+(* In case of failure, the state is backtracked. *)
+Definition mapStateT2
+  {S A : UU0} {M : monad}
+  (f : M (A*S)%type -> M (A*S)%type -> M (A*S)%type) (m1 m2 : stateT S M A) :
+stateT S M A :=
+fun s => f (runStateT m1 s) (runStateT m2 s).
+
+Section FastProduct.
+
+Local Obligation Tactic := idtac.
+Local Set Bullet Behavior "Strict Subproofs".
+
+Variable M : exceptMonad.
+Let N : monad := stateT nat M.
+
+Fixpoint fastProductRec (xs : list nat) : N unit :=
+match xs with
+| nil => Ret tt
+| cons 0 _ => Lift (stateT nat) M unit Fail
+| cons (S x) xs' => Get >>= fun r => Put (r * S x) >> fastProductRec xs'
+end.
+
+Definition fastProduct (xs : list nat) : N nat :=
+mapStateT2 Catch (Put 1 >> fastProductRec xs >> Get) (Ret 0).
+
+Require Import Arith.
+Import Nat.
+
+Lemma fastProductCorrect (xs : list nat) (s : nat) :
+evalStateT (fastProduct xs) s = Ret (product xs).
+Proof.
+assert (Hgen : forall n,
+  evalStateT (mapStateT2 Catch ((Put n >> fastProductRec xs) >> Get)
+     (Ret 0)) s = Ret (n * product xs)).
+{
+  induction xs as [ | [ | x] xs IH]; cbn; intro n.
+  - rewrite mult_1_r bindA bindretf putget.
+    unfold mapStateT2, evalStateT.
+    rewrite runStateTFun runStateTBind runStateTPut bindretf runStateTRet
+     catchret bindretf.
+    reflexivity.
+  - rewrite mult_0_r.
+    unfold mapStateT2, evalStateT.
+    rewrite runStateTFun runStateTBind runStateTBind runStateTPut bindretf
+     runStateTLfail bindfailf catchfailm runStateTRet bindretf.
+    reflexivity.
+  - rewrite <- bindA.
+    rewrite putget bindA bindA bindretf.
+    rewrite <- bindA, <- bindA, putput, IH.
+    rewrite <- mult_n_Sm, mult_comm, mul_add_distr_l, mul_add_distr_l,
+     plus_comm, mult_comm, (mult_comm (product xs)), mult_assoc.
+    reflexivity.
+}
+rewrite Hgen.
+cbn.
+by rewrite <- plus_n_O.
+Qed.
+
+End FastProduct.
+
+(* The following example illustrates how the state is backtracked when a
+   failure is catched. *)
+Goal
+runStateT (
+  Put 1 >>
+  mapStateT2 Catch (Put 2 >> Lift (stateT _) ModelExcept.t _ Fail) Get) 0 =
+inr (1, 1).
+Proof.
+rewrite runStateTBind runStateTPut bindretf.
+unfold mapStateT2.
+rewrite runStateTFun runStateTBind runStateTPut bindretf runStateTLfail
+ catchfailm runStateTGet.
+reflexivity.
+Qed.
+
+(* The following fail-state monad is such that it does not backtrack the
+   state. *)
+Section PersistentState.
+
+Variable S : UU0.
+
+Definition failPState (A : UU0) : UU0 :=
+S -> option A * S.
+
+Definition runFailPState {A : UU0} (m : failPState A) (s : S) : option A * S :=
+m s.
+
+Definition ret {A : UU0} (a : A) : failPState A :=
+fun s => (Some a, s).
+
+Definition bind {A B : UU0} (m : failPState A) (f : A -> failPState B) :
+failPState B :=
+fun s => match m s with
+| (None, s') => (None, s')
+| (Some a, s') => f a s'
+end.
+
+Lemma bindretf (A B : UU0) (a : A) (f : A -> failPState B) :
+bind (ret a) f = f a.
+Proof.
+reflexivity.
+Qed.
+
+Lemma bindmret (A : UU0) (m : failPState A) :
+bind m ret = m.
+Proof.
+apply fun_ext => s.
+unfold bind.
+destruct (m s) as [[|]]; reflexivity.
+Qed.
+
+Lemma bindA
+  (A B C : UU0) (m : failPState A)
+  (f : A -> failPState B) (g : B -> failPState C) :
+bind (bind m f) g = bind m (fun x => bind (f x) g).
+Proof.
+apply fun_ext => s.
+unfold bind.
+destruct (m s) as [[|]]; reflexivity.
+Qed.
+
+Definition fail {A : UU0} : failPState A := fun s => (None, s).
+
+Definition catch {A : UU0} (m1 m2 : failPState A) :=
+fun s => match m1 s with
+| (Some a, s') => (Some a, s')
+| (None, s') => m2 s'
+end.
+
+Definition get : failPState S := fun s => (Some s, s).
+
+Definition put (s : S) : failPState unit := fun _ => (Some tt, s).
+
+End PersistentState.
+
+Arguments runFailPState {_ _} _ _.
+Arguments ret {_ _} _.
+Arguments bind {_ _ _} _ _.
+Arguments fail {_ _}.
+Arguments get {_}.
+Arguments put {_} _.
+
+Local Notation "m >>> f" := (bind m (fun _ => f)) (at level 49).
+
+(* The following example illustrates how the state is NOT backtracked when a
+   failure is catched. *)
+Goal
+  runFailPState (put 1 >>> catch (put 2 >>> fail) get) 0 =
+  (Some 2, 2).
+Proof.
+reflexivity.
+Qed.
